coq/Proofs/Tactics.v
@@ -131,6 +131,7 @@ Ltac bool_inv :=
 Ltac bool_to_prop_hyp :=
   repeat match goal with
     | [H: orb _ _ = false |- _] => apply orb_false_elim in H; destruct H
+    | [H: orb _ _ = true |- _] =>  apply orb_prop in H; destruct H
     | [H: andb _ _ = true |- _] => apply andb_prop in H; destruct H
     | [H: andb _ _ = false |- _] => apply andb_false_iff in H; destruct H
     | [H: Z.eqb _ _ = true |-_] => apply Z.eqb_eq in H
